Let's consider the following code.

```py
def test(n):
    if n>0:
        print(n)
        test(n-1)
```

Output

```
3
2
1
```

T(n): Total amount of time taken for recursive function

```py
def test(n):        # T(n): total amount of time taken
    if n>0:
        print(n)    # 1
        test(n-1)   # T(n-1)
```

If `test(n)`'s time complexity is `T(n)`, then `test(n-1)`'s time complexity is `T(n-1)`,

therefore, `T(n) = T(n-1) + 1`

# How to find T(n) for general k steps

Given the following equation,

`T(n) = T(n-1) + 1`

Now let's find the T(n) in terms of k times.

First, we need to find the pattern, so let's assume that k=1

1.

Express T(n-1) in terms of T(n-2).

T(n-1) = T(n - 1 - 1) + 1 = `T(n-2) + 1`

2. 

Substitute the expression back into the original equation,

T(n) = T(n-2) + 1 + 1 = `T(n-2) + 2`

3. 

Generalize for k iterations.

We can continue this substitution process iteratively to generalize it for k steps, eventually arriving at:

`T(n) = T(n-k) + k`

4.

We assume that n-k = 0, so `n = k`.

`T(n) = T(n-n) + n = T(0) + n = 1 + n`

Therefore `T(n) = n`
